complete decode base case

Varint.fst
@@ -26,41 +26,11 @@ let rec valid (v:list UInt8.t) : bool =
        which is equivalent to the number fitting into 7 bits *)
   | msb :: [] -> UInt.fits (U8.v msb) 7
     (* Otherwise the continuation bit should be one *)
-    (* Note that U.msb is "most significant bit" while the msb in the pattern match is "most significant byte" *)
+    (* Note that U.msb is "most significant bit" while the msb in the pattern is "most significant byte" *)
   | msb :: rest -> U.msb (U8.v msb) && valid rest
 
 let varint = v:list UInt8.t{length v >= 1 /\ valid v}
 
-let zero_extend_m_vec (#n:pos) (a:BitVector.bv_t n) (m:pos): Tot (BitVector.bv_t (n+m)) = 
-  Seq.append (create m false) a
-
-let zero_extend_m (#n:pos) (a:uint_t n) (m:pos): Tot (uint_t (n+m)) = 
-  from_vec (zero_extend_m_vec (to_vec a) m)
-
-val logand_append: #n:pos -> #m:pos -> a:BitVector.bv_t n -> b:BitVector.bv_t n -> 
-                    c:BitVector.bv_t m -> d:BitVector.bv_t m ->
-                    Lemma (ensures Seq.append (BitVector.logand_vec a b) (BitVector.logand_vec c d) =
-                                   BitVector.logand_vec #(n+m) (Seq.append a c) (Seq.append b d))
-
-val logand_trunc_lemma: #n:pos -> a:uint_t n -> m:pos ->
-  Lemma (requires U.size a m /\ m <= n) (ensures (U.logand a (U.to_uint_t n (U.max_int m))) = a)
-
-let logand_trunc_lemma #n a m = 
-  let b = U.max_int m in
-  let b' = U.to_uint_t m b in
-  let b'' = U.to_uint_t n b in
-  let a' = U.to_uint_t m a in
-  FStar.Math.Lemmas.pow2_le_compat n m;
-  FStar.Math.Lemmas.modulo_lemma b (pow2 n);
-  FStar.Math.Lemmas.modulo_lemma b (pow2 m);
-  assert b' = b'';
-  FStar.Math.Lemmas.modulo_lemma a (pow2 m);
-  assert a = a';
-  UInt.logand_lemma_2 a';
-  assert U.logand a b'' = a;
-  assert True
-  
-  
 #push-options "--split_queries always"
 
 let rec encode (x: U64.t) : Tot varint (decreases (U64.v x)) = 
@@ -85,21 +55,59 @@ let rec encode (x: U64.t) : Tot varint (decreases (U64.v x)) =
     assert (U8.v nextByte) >= 128;
     UInt.lemma_msb_pow2 (U8.v nextByte);
     let enc = List.append [nextByte] restEnc in 
-    assert length enc > 1;
     enc
 
-#pop-options
+
+val lemma_varint_max (bs:varint) (x: U64.t) : 
+  Lemma (requires bs = encode x) (ensures UInt.fits (U64.v x) (7 * length bs))
+let rec lemma_varint_max bs x = 
+  match bs with 
+  | msb :: [] -> let nextByte = U64.logand x 0x7FuL in
+               let nextByte' = Cast.uint64_to_uint8 nextByte in
+               UInt.logand_le (U64.v x) 0x7F;
+               assert UInt.fits (U64.v nextByte) 7;
+               assert [msb] = [nextByte'];
+               assert op_Division (U64.v x) 128 = 0; 
+               ()
+  | msb :: rest -> assume False; ()
+
+val lemma_varint_max' (bs:varint) : 
+  Lemma (exists x. bs = encode x /\ UInt.fits (U64.v x) (7 * length bs))
+let lemma_varint_max' bs = assume False
 
 let rec decode (bs:varint) (x:erased U64.t{bs = encode(reveal x)}) : y:U64.t{y = reveal x} =
+  match bs with 
+  | msb :: [] -> 
+            assert UInt.fits (U8.v msb) 7;
+            UInt.logand_le (U64.v x) 0x7F;
+            lemma_varint_max bs x;
+            assert U64.v (reveal x) < 128;
+            UInt.logand_mask (U64.v x) 7;
+            FStar.Math.Lemmas.modulo_lemma (U64.v x) 128;
+            FStar.Math.Lemmas.modulo_lemma (U64.v x) 256;
+            Cast.uint8_to_uint64 msb
+  | msb :: rest -> let msx = U64.(Cast.uint8_to_uint64 msb |^ 128uL) in
+                 assume rest = encode U64.(x |^ msx);
+                 let rx = decode rest U64.(x |^ msx) in 
+                 assume False;
+                 U64.(msx +^ rx <<^ 7ul)
+
+let rec decode' (bs:varint) (x:erased U64.t{bs = encode(reveal x)}) : y:U64.t{y = reveal x} =
   let nextByte = hd bs in
   match U.msb (U8.v nextByte) with 
   | false -> assert length bs = 1; 
+            assert UInt.fits (U8.v nextByte) 7;
             UInt.logand_le (U64.v x) 0x7F;
-            assert U64.(v (x >>^ 7ul)) <= 0;
+            lemma_varint_max bs x;
             assert U64.v (reveal x) < 128;
-            assert nextByte = Cast.uint64_to_uint8 (U64.logand (reveal x) 0x7FuL);
-            assert U8.v nextByte = U64.v (reveal x);
+            UInt.logand_mask (U64.v x) 7;
+            FStar.Math.Lemmas.modulo_lemma (U64.v x) 128;
+            FStar.Math.Lemmas.modulo_lemma (U64.v x) 256;
             Cast.uint8_to_uint64 nextByte
-  | true -> 0uL
+  | true ->  assert length bs > 1; 
+            let rest : varint = tl bs in
+            let nextByte' = U8.(nextByte -^ 128uy) in
+            assume False; 0uL 
   
+#pop-options
 (* Relevant F* code in ASN1*: ANS1.Spec.IdentifierU32.fst *)
